src/cbor/spec/raw/CBOR.Spec.Raw.Optimal.fst
@@ -1,0 +1,93 @@
+module CBOR.Spec.Raw.Optimal
+include CBOR.Spec.Raw.Valid2
+open CBOR.Spec.Util
+open FStar.Mul
+
+module U8 = FStar.UInt8
+module U64 = FStar.UInt64
+
+(* Shortest-size integers *)
+
+let raw_uint64_optimal (x: raw_uint64) : Tot bool =
+  ((U64.v x.value <= U8.v max_simple_value_additional_info) = (U8.v x.size = 0)) &&
+  begin
+    if U8.v x.size <= 1
+    then true
+    else pow2 (8 * pow2 (U8.v x.size - 2)) <= U64.v x.value
+  end
+
+let raw_uint64_optimal_unique (x1 x2: raw_uint64) : Lemma
+  (requires (raw_uint64_optimal x1 /\ raw_uint64_optimal x2 /\ raw_uint64_equiv x1 x2))
+  (ensures (x1 == x2))
+= ()
+
+let mk_raw_uint64 (x: U64.t) : Pure raw_uint64
+  (requires True)
+  (ensures (fun y -> y.value == x /\
+    raw_uint64_optimal y == true
+  ))
+= let size =
+    if U64.lte x (FStar.Int.Cast.uint8_to_uint64 max_simple_value_additional_info)
+    then 0uy
+    else if U64.lt x 256uL
+    then 1uy
+    else if U64.lt x 65536uL
+    then 2uy
+    else if U64.lt x 4294967296uL
+    then 3uy
+    else 4uy
+  in
+  { size = size; value = x }
+
+let raw_uint64_optimize (x: raw_uint64) : Pure raw_uint64
+  (requires True)
+  (ensures (fun x' -> raw_uint64_equiv x x' /\ raw_uint64_optimal x'))
+= mk_raw_uint64 x.value
+
+let raw_data_item_ints_optimal_elem (x: raw_data_item) : Tot bool =
+  match x with
+  | Int64 _ v
+  | String _ v _
+  | Array v _
+  | Map v _
+  | Tagged v _
+    -> raw_uint64_optimal v
+  | Simple _ -> true
+
+let raw_data_item_ints_optimal : raw_data_item -> Tot bool =
+  holds_on_raw_data_item raw_data_item_ints_optimal_elem
+
+let raw_data_item_uint64_optimize_elem (x: raw_data_item) : Tot raw_data_item =
+  match x with
+  | Int64 ty v -> Int64 ty (raw_uint64_optimize v)
+  | String ty len v -> String ty (raw_uint64_optimize len) v
+  | Array len v -> Array (raw_uint64_optimize len) v
+  | Map len v -> Map (raw_uint64_optimize len) v
+  | Tagged tag v -> Tagged (raw_uint64_optimize tag) v
+  | _ -> x
+
+(*
+let raw_data_item_uint64_optimize_elem_valid (x: raw_data_item) : Lemma
+  (requires (valid basic_data_model x == true))
+  (ensures (valid basic_data_model (raw_data_item_uint64_optimize_elem x) == true /\
+    raw_equiv2 x (raw_data_item_uint64_optimize_elem x) == true
+  ))
+= valid_eq basic_data_model x;
+  valid_eq basic_data_model (raw_data_item_uint64_optimize_elem x);
+  equiv_eq basic_data_model x (raw_data_item_uint64_optimize_elem x);
+  match x with
+  | Array _ v ->
+    list_for_all2_refl raw_equiv2 v (fun x -> equiv_refl basic_data_model x)
+  | Map _ v ->
+    list_for_all_intro (setoid_assoc_eq raw_equiv2 raw_equiv2 v) v (fun y ->
+      equiv_refl basic_data_model (fst y);
+      list_setoid_assoc_mem_elim raw_equiv2 v y (fst y);
+      let Some y' = list_setoid_assoc raw_equiv2 (fst y) v in
+      
+      equiv_refl basic_data_model y';
+      ()
+    );
+    ()
+  | Tagged _ v -> equiv_refl basic_data_model v
+  | _ -> ()
+
